src/model.lean
@@ -31,83 +31,79 @@ private lemma vecterm.equiv_trans (T : theory L) : ∀ {n} {v₁ v₂ v₃ : vec
 | (n+1) (vecterm.cons t₁ v₁) (vecterm.cons t₂ v₂) (vecterm.cons t₃ v₃) := 
     by {simp[vecterm.equiv], refine λ e₁ h₁ e₂ h₂, ⟨provable.eq_trans e₁ e₂, vecterm.equiv_trans h₁ h₂⟩ }
 
-theorem vecterm_equiv_equivalence (T : theory L) (n) : equivalence (vecterm.equiv T n) :=
-⟨vecterm.equiv_refl T, λ _ _ , vecterm.equiv_symm T, λ _ _ _, vecterm.equiv_trans T⟩
+theorem vecterm_equiv_equivalence (T : theory L) : equivalence (λ t₁ t₂, T ⊢̇ t₁ =̇ t₂) :=
+⟨λ _, by simp, λ _ _ , provable.eq_symm.mp, λ _ _ _, provable.eq_trans⟩
 
-def Herbrand (n) : Type u :=
-quotient (⟨vecterm.equiv T n, vecterm_equiv_equivalence T n⟩ : setoid (vecterm L n))
+@[reducible, simp, instance]
+def herbrand : setoid (term L) := ⟨λ t₁ t₂, T ⊢̇ t₁ =̇ t₂, vecterm_equiv_equivalence T⟩
 
-def vecterm.quo (T : theory L) {n} (t : vecterm L n) : Herbrand T n := quotient.mk' t
+def Herbrand : Type u := quotient (herbrand T)
+
+def vecterm.quo (T : theory L) (t : term L) : Herbrand T := quotient.mk' t
 
 notation `⟦`v`⟧ᵗ.`T :max := vecterm.quo T v
+local infix ` ≋ `:80 := (@setoid.vec_r _ (herbrand T) _)
 
-instance (T : theory L) : inhabited (Herbrand T 0) := ⟨⟦#0⟧ᵗ.T⟩
+instance (T : theory L) : inhabited (Herbrand T) := ⟨⟦#0⟧ᵗ.T⟩
 
 namespace Herbrand
 variables {T}
 
 @[elab_as_eliminator]
-protected lemma ind_on {n} {C : Herbrand T n → Prop} (d : Herbrand T n)
-  (h : ∀ t : vecterm L n, C ⟦t⟧ᵗ.T) : C d :=
+protected lemma ind_on {C : Herbrand T → Prop} (d : Herbrand T)
+  (h : ∀ t : term L, C ⟦t⟧ᵗ.T) : C d :=
 quotient.induction_on' d h
 
 @[elab_as_eliminator, reducible]
-protected def lift_on {φ} {n} (d : Herbrand T n) (f : vecterm L n → φ)
-  (h : ∀ v u : vecterm L n, v ≃[T] u → f v = f u) : φ :=
+protected def lift_on {φ} (d : Herbrand T) (f : term L → φ)
+  (h : ∀ v u : term L, T ⊢̇ v =̇ u → f v = f u) : φ :=
 quotient.lift_on' d f h
 
 @[simp]
-protected lemma lift_on_eq {φ} {n} (t : vecterm L n) (f : vecterm L n → φ)
-  (h : ∀ v u, v ≃[T] u → f v = f u) : fopl.Herbrand.lift_on ⟦t⟧ᵗ.T f h = f t := rfl
+protected lemma lift_on_eq {φ} (t : term L) (f : term L → φ)
+  (h : ∀ v u, T ⊢̇ v =̇ u → f v = f u) : fopl.Herbrand.lift_on ⟦t⟧ᵗ.T f h = f t := rfl
 
 @[elab_as_eliminator, reducible, simp]
-protected def lift_on₂ {φ} {n} (d₁ d₂ : Herbrand T n) (f : vecterm L n → vecterm L n → φ)
-  (h : ∀ t₁ t₂ u₁ u₂, (t₁ ≃[T] u₁) → (t₂ ≃[T] u₂) → f t₁ t₂ = f u₁ u₂) : φ :=
+protected def lift_on₂ {φ} (d₁ d₂ : Herbrand T) (f : term L → term L → φ)
+  (h : ∀ t₁ t₂ u₁ u₂, (T ⊢̇ t₁ =̇ u₁) → (T ⊢̇ t₂ =̇ u₂) → f t₁ t₂ = f u₁ u₂) : φ :=
 quotient.lift_on₂' d₁ d₂ f h
 
 @[simp]
-protected lemma lift_on₂_eq {φ} {n} (t u : vecterm L n) (f : vecterm L n → vecterm L n → φ)
-  (h : ∀ t₁ t₂ u₁ u₂, (t₁ ≃[T] u₁) → (t₂ ≃[T] u₂) → f t₁ t₂ = f u₁ u₂) :
+protected lemma lift_on₂_eq {φ} (t u : term L) (f : term L → term L → φ)
+  (h : ∀ t₁ t₂ u₁ u₂, (T ⊢̇ t₁ =̇ u₁) → (T ⊢̇ t₂ =̇ u₂) → f t₁ t₂ = f u₁ u₂) :
   fopl.Herbrand.lift_on₂ ⟦t⟧ᵗ.T ⟦u⟧ᵗ.T f h = f t u := rfl
 
-#check quotient.lift
-
-@[simp] lemma of_eq_of {n} {t u : vecterm L n} : ⟦t⟧ᵗ.T = ⟦u⟧ᵗ.T ↔ (t ≃[T] u) :=
+@[simp] lemma of_eq_of {t u : term L} : ⟦t⟧ᵗ.T = ⟦u⟧ᵗ.T ↔ (T ⊢̇ t =̇ u) :=
 by simp[vecterm.quo, vecterm.equiv, quotient.eq']
 
-def dvector.cons'_aux (T : theory L) (t : term L) : ∀ n, Herbrand T n → Herbrand T (n+1) :=
-λ n p, Herbrand.lift_on p (λ v, ⟦vecterm.cons t v⟧ᵗ.T) $
-  λ p₁ p₂ hyp, by simp* at*
+@[elab_as_eliminator, reducible]
+protected def lift_on_vec {φ} {n} (v : dvector (Herbrand T) n) (f : dvector (term L) n → φ)
+  (h : ∀ (a b : dvector (term L) n), a ≋ b → f a = f b) : φ :=
+quotient.lift_on_vec v f h
 
-def dvector.cons' : ∀ {n}, Herbrand T 0 → Herbrand T n → Herbrand T (n+1) :=
-λ n t, Herbrand.lift_on t (λ t, dvector.cons'_aux T t n) $
-  λ t₁ t₂ hyp, by { simp, funext e, induction e using fopl.Herbrand.ind_on,
-  simp[dvector.cons'_aux], refine hyp }
-
-def dvector_to_herbrand : ∀ {n}, dvector (Herbrand T 0) (n+1) → Herbrand T n
-| 0     c        := c.head
-| (n+1) (a :: v) := dvector.cons' a (dvector_to_herbrand v)
+@[simp]
+protected lemma lift_on_vec_eq {φ} {n} (u : dvector (term L) n) (f : dvector (term L) n → φ)
+  (h : ∀ (v u : dvector (term L) n), v ≋ u → f v = f u) :
+fopl.Herbrand.lift_on_vec ᵥ⟦u⟧ f h = f u := quotient.lift_on_vec_eq u f h
 
 def symbol.pconstant (c : L.pr 0) : Prop := T ⊢̇ form.const c
 
-def symbol.fn' {n} (f : L.fn (n+1)) : Herbrand T n → Herbrand T 0 :=
-λ e, Herbrand.lift_on e (λ v, ⟦vecterm.app f v⟧ᵗ.T) $
-  λ t₁ t₂ hyp, by { simp* at*,
-  refine (show T ⊢̇ t₁ ≡̇ t₂ →̇ vecterm.app f t₁ =̇ vecterm.app f t₂, by simp).MP hyp }
+@[simp] lemma equivs_equals : ∀ {n} (v₁ v₂ : dvector (term L) (n+1)),
+  v₁ ≋ v₂ ↔ (T ⊢̇ v₁.to_vecterm ≡̇ v₂.to_vecterm)
+| 0 (t₁ :: dvector.nil) (t₂ :: dvector.nil) := by { simp, refl }
+| (n+1) (t₁ :: v₁) (t₂ :: v₂) := by { simp[equivs_equals v₁ v₂], intros, refl }
 
-def symbol.fn : ∀ {n} (f : L.fn n), dvector (Herbrand T 0) n → Herbrand T 0
+def symbol.fn : ∀ {n} (f : L.fn n), dvector (Herbrand T) n → Herbrand T
 | 0     c _ := ⟦vecterm.const c⟧ᵗ.T
-| (n+1) f v := symbol.fn' f (dvector_to_herbrand v)
+| (n+1) f v := fopl.Herbrand.lift_on_vec v (λ u : dvector (term L) (n+1), ⟦vecterm.app f (u.to_vecterm)⟧ᵗ.T) 
+  $ λ v₁ v₂ eqn, by { simp at*, refine provable.e4.MP eqn }
 
-def symbol.pr' {n} (p : L.pr (n+1)) : Herbrand T n → Prop :=
-λ e, Herbrand.lift_on e (λ v, T ⊢̇ form.app p v) $
-  λ t₁ t₂ hyp, by { simp[-provable.iff],  }
-
-def symbol.pr : ∀ {n} (f : L.pr n), dvector (Herbrand T 0) n → Prop
+def symbol.pr : ∀ {n} (f : L.pr n), dvector (Herbrand T) n → Prop
 | 0     c _ := T ⊢̇ form.const c
-| (n+1) p v := symbol.pr' p (dvector_to_herbrand v)
+| (n+1) p v := fopl.Herbrand.lift_on_vec v (λ u : dvector (term L) (n+1), T ⊢̇ form.app p (u.to_vecterm))
+  $ λ v₁ v₂ eqn, by { simp at*, refine ⟨(provable.e5.MP eqn).MP, (provable.e5.MP (vecterm.equiv_symm _ eqn)).MP⟩  }
 
-def model (T : theory L) : model L := ⟨Herbrand T 0, ⟦#0⟧ᵗ.T, @symbol.fn _ T, @symbol.pr _ T⟩
+def model (T : theory L) : model L := ⟨Herbrand T, ⟦#0⟧ᵗ.T, @symbol.fn _ T, @symbol.pr _ T⟩
 notation `𝔗[`T`]` := model T
 
 end Herbrand
@@ -130,6 +126,7 @@ def form.quo (T : theory L) (p : form L) : Lindenbaum T := quotient.mk' p
 notation `⟦`p`⟧.`T :max := form.quo T p
 
 namespace Lindenbaum
+open provable
 variables {T}
 
 @[elab_as_eliminator]
@@ -164,6 +161,8 @@ instance : has_le (Lindenbaum T) :=
  λ p₁ p₂ q₁ q₂ hp hq, by { simp at*,
    exact ⟨λ h, (hp.2.imp_trans h).imp_trans hq.1, λ h, (hp.1.imp_trans h).imp_trans hq.2⟩ }⟩
 
+instance : has_lt (Lindenbaum T) := ⟨λ l k, l ≤ k ∧ ¬k ≤ l⟩
+
 def imply : Lindenbaum T → Lindenbaum T → Lindenbaum T :=
 λ p₁ p₂, Lindenbaum.lift_on₂ p₁ p₂ (λ p₁ p₂, ⟦p₁ →̇ p₂⟧.T) $
  λ p₁ p₂ q₁ q₂ hp hq, by { simp at*, split,
@@ -175,7 +174,7 @@ def imply : Lindenbaum T → Lindenbaum T → Lindenbaum T :=
      have : T+{q₁ →̇ q₂}+{p₁} ⊢̇ q₁, from (show _ ⊢̇ p₁ →̇ q₁, by simp[hp]).MP (by simp),
      have : T+{q₁ →̇ q₂}+{p₁} ⊢̇ q₂, from (show _ ⊢̇ q₁ →̇ q₂, by simp).MP this,
      exact (show _ ⊢̇ q₂ →̇ p₂, by simp[hq]).MP this  } }
-infixr ` ⊐ `:60 := imply
+infixr ` ⊳ `:60 := imply
 
 instance : has_mul (Lindenbaum T) :=
 ⟨λ p₁ p₂, Lindenbaum.lift_on₂ p₁ p₂ (λ p₁ p₂, ⟦p₁ ⩑ p₂⟧.T) $
@@ -226,6 +225,28 @@ def ex : Lindenbaum ⇑T → Lindenbaum T := λ p, Lindenbaum.lift_on p (λ p, �
     exact lmm₂.MP lmm₁ }
 prefix `∐`:90 := ex
 
+@[simp] def predicate : ∀ {n} (f : L.pr n), dvector (Herbrand T) n → Lindenbaum T
+| 0     c _ := ⟦form.const c⟧.T
+| (n+1) p v := fopl.Herbrand.lift_on_vec v (λ u : dvector (term L) (n+1), ⟦form.app p (u.to_vecterm)⟧.T)
+  $ λ v₁ v₂ eqn, by { simp at*, refine ⟨provable.e5.MP eqn, provable.e5.MP (vecterm.equiv_symm _ eqn)⟩ }
+
+def predicate₁ (f : L.pr 1) (h : Herbrand T) : Lindenbaum T := predicate f (h :: dvector.nil)
+
+def predicate₂ (f : L.pr 2) (h₁ h₂ : Herbrand T) : Lindenbaum T := predicate f (h₁ :: h₂ :: dvector.nil)
+
+def equal : Herbrand T → Herbrand T → Lindenbaum T :=
+λ h₁ h₂, fopl.Herbrand.lift_on₂ h₁ h₂ (λ t₁ t₂, ⟦t₁ =̇ t₂⟧.T) $
+λ t₁ t₂ u₁ u₂ eqn₁ eqn₂, by { simp, refine ⟨provable.deduction.mp _, provable.deduction.mp  _⟩,
+  have lmm₁ : T+{t₁ =̇ t₂} ⊢̇ u₁ =̇ t₁, simp [provable.e2.MP eqn₁],
+  have lmm₂ : T+{t₁ =̇ t₂} ⊢̇ t₁ =̇ t₂, simp,
+  have lmm₃ : T+{t₁ =̇ t₂} ⊢̇ t₂ =̇ u₂, simp [eqn₂],
+  refine (lmm₁.eq_trans lmm₂).eq_trans lmm₃,
+  have lmm₁ : T+{u₁ =̇ u₂} ⊢̇ t₁ =̇ u₁, simp [eqn₁],
+  have lmm₂ : T+{u₁ =̇ u₂} ⊢̇ u₁ =̇ u₂, simp,
+  have lmm₃ : T+{u₁ =̇ u₂} ⊢̇ u₂ =̇ t₂, simp [provable.e2.MP eqn₂],
+  refine (lmm₁.eq_trans lmm₂).eq_trans lmm₃ }
+infix ` ⋈ `:80 := equal
+
 def sf : Lindenbaum T → Lindenbaum ⇑T := λ p, Lindenbaum.lift_on p (λ p, ⟦p.sf⟧.⇑T) $
 λ p₁ p₂ hyp, by { simp[form.ex, provable.contrapose] at*, have := provable.dummy_fal_quantifir_iff, }
 
@@ -243,32 +264,48 @@ begin
   simp[has_le.le], refine λ h₁ h₂, ⟨h₁, h₂⟩
 end
 
+lemma imply_le {l k : Lindenbaum T} : l ⊳ k = 1 ↔ l ≤ k :=
+
+
 lemma provable_GE {l : Lindenbaum ⇑T} : □l → □∏l :=
 by { induction l using fopl.Lindenbaum.ind_on, simp[fal, provable], exact provable.GE }
 
-lemma provable_K {l k : Lindenbaum T} : □(l ⊐ k) → □l → □k :=
+lemma provable_AX {p} (h : p ∈ T) : ⟦p⟧.T = 1 :=
+by simp[has_one.one, provable.AX h]
+
+lemma provable_K {l k : Lindenbaum T} : □(l ⊳ k) → □l → □k :=
 begin
   induction l using fopl.Lindenbaum.ind_on,
   induction k using fopl.Lindenbaum.ind_on,
   simp[imply, provable], refine λ h₁ h₂, h₁.MP h₂
 end
 
+@[simp] lemma equal_refl {h : Herbrand T}  : h ⋈ h = 1 :=
+by induction h using fopl.Herbrand.ind_on; simp[equal, has_one.one]
+
+@[simp] lemma equal_subst₁ {h₁ h₂ : Herbrand T} {p : L.pr 1} : h₁ ⋈ h₂ ≤ predicate₁ p h₁ ⊳ predicate₁ p h₂ :=
+by { induction h₁ using fopl.Herbrand.ind_on, induction h₂ using fopl.Herbrand.ind_on,
+      simp[equal, has_le.le, imply, has_one.one, predicate₁,
+        (show ⟦h₁⟧ᵗ.T :: dvector.nil = ᵥ⟦h₁ :: dvector.nil⟧, by refl),
+        (show ⟦h₂⟧ᵗ.T :: dvector.nil = ᵥ⟦h₂ :: dvector.nil⟧, by refl) ], 
+        }
+
 lemma double_inv (l : Lindenbaum T) : l⁻¹⁻¹ = l :=
 by induction l using fopl.Lindenbaum.ind_on; simp[has_inv.inv]
 
 #check provable.prenex_fal_quantifir_imp1 _ _
 
-lemma prenex_fal_quantifir_imp1  {l : Lindenbaum ⇑T} {k : Lindenbaum T} : ∏l ⊐ k = ∐(l ⊐ k.sf) := by sorry
+lemma prenex_fal_quantifir_imp1  {l : Lindenbaum ⇑T} {k : Lindenbaum T} : ∏l ⊳ k = ∐(l ⊳ k.sf) := by sorry
 
 lemma prenex_fal_quantifir_neg  {l : Lindenbaum ⇑T} : (∏l)⁻¹ = ∐l⁻¹  := by sorry
 
 @[simp] lemma provable_one : □(1 : Lindenbaum T) :=
 by simp[has_one.one, provable]
 
-@[simp] lemma one_maximum {l : Lindenbaum T} : l ≤ 1 :=
+@[simp] lemma one_maximum (l : Lindenbaum T) : l ≤ 1 :=
 by induction l using fopl.Lindenbaum.ind_on; simp[has_one.one, has_le.le]
 
-@[simp] lemma zero_minimum {l : Lindenbaum T} : 0 ≤ l :=
+@[simp] lemma zero_minimum (l : Lindenbaum T) : 0 ≤ l :=
 by induction l using fopl.Lindenbaum.ind_on; simp[has_zero.zero, has_le.le]
 
 lemma Box_iff {l : Lindenbaum T} : □l ↔ l = 1 :=
@@ -292,6 +329,94 @@ by { induction l using fopl.Lindenbaum.ind_on, induction k using fopl.Lindenbaum
 lemma add_le_r {l k : Lindenbaum T} : k ≤ l + k :=
 by { induction l using fopl.Lindenbaum.ind_on, induction k using fopl.Lindenbaum.ind_on,
      simp[has_add.add, has_le.le, provable.or_r] }
+
+private lemma sup_le {l m n : Lindenbaum T} : l ≤ n → m ≤ n → l + m ≤ n :=
+by { induction l using fopl.Lindenbaum.ind_on,
+       induction m using fopl.Lindenbaum.ind_on,
+       induction n using fopl.Lindenbaum.ind_on, simp[has_le.le, has_add.add],
+       intros h₁ h₂, exact provable.hyp_or h₁ h₂   }
+
+private lemma le_inf {l m n : Lindenbaum T} : l ≤ m → l ≤ n → l ≤ m * n :=
+by { induction l using fopl.Lindenbaum.ind_on,
+     induction m using fopl.Lindenbaum.ind_on,
+     induction n using fopl.Lindenbaum.ind_on,
+     simp[has_le.le, has_mul.mul],
+     refine λ h₁ h₂, provable.deduction.mp _, simp,
+     refine ⟨provable.deduction.mpr h₁, provable.deduction.mpr h₂⟩  }
+
+private lemma le_sup_inf {l m n : Lindenbaum T} : (l + m) * (l + n) ≤ l + m * n :=
+by { induction l using fopl.Lindenbaum.ind_on,
+     induction m using fopl.Lindenbaum.ind_on,
+     induction n using fopl.Lindenbaum.ind_on,
+     simp[has_add.add, has_mul.mul, has_le.le, provable.or_r, form.or],
+     refine provable.deduction.mp (provable.deduction.mp _),
+     have lmm₁ : T+{(¬̇l →̇ m) ⩑ (¬̇l →̇ n)}+{¬̇l} ⊢̇ (¬̇l →̇ m) ⩑ (¬̇l →̇ n), simp[-provable.and],
+     have lmm₂ : T+{(¬̇l →̇ m) ⩑ (¬̇l →̇ n)}+{¬̇l} ⊢̇ ¬̇l, simp,
+     simp at lmm₁ ⊢, refine ⟨lmm₁.1.MP lmm₂, lmm₁.2.MP lmm₂⟩ }
+
+
+private lemma sup_inf_sdiff (l m : Lindenbaum T) : l * m + l * m⁻¹ = l :=
+by { induction l using fopl.Lindenbaum.ind_on, induction m using fopl.Lindenbaum.ind_on,
+      simp[has_le.le, has_add.add, has_mul.mul, has_inv.inv, has_one.one, form.or],
+      refine ⟨contrapose.mp (deduction.mp _), _⟩, simp,
+      have : ∀ n, T+{¬̇l} ⊢̇ ¬̇(l ⩑ n),
+      { refine λ n, deduction.mpr (contrapose.mpr (deduction.mp _)),
+        have : T+{l ⩑ n} ⊢̇ l ⩑ n, simp[-provable.and], simp* at* },
+      refine ⟨this _, this _⟩,
+      refine deduction.mp (deduction.mp _), simp, refine neg_hyp (deduction.mp _),
+      refine explosion (show T+{l}+{¬̇(l ⩑ m)}+{m} ⊢̇ l ⩑ m, by simp) (by simp) }
+
+private lemma inf_inf_sdiff (l m : Lindenbaum T) : l * m * (l * m⁻¹) = 0 :=
+by { induction l using fopl.Lindenbaum.ind_on, induction m using fopl.Lindenbaum.ind_on,
+     simp[has_le.le, has_add.add, has_mul.mul, has_inv.inv, has_zero.zero, form.or],
+     refine deduction.mp (explosion (show T+{l ⩑ m ⩑ (l ⩑ ¬̇m)} ⊢̇ m, by simp[axiom_and]) (by simp[axiom_and])) }
+
+private lemma inf_compl_le_bot (l : Lindenbaum T) : l * l⁻¹ ≤ 0 :=
+by { induction l using fopl.Lindenbaum.ind_on, simp[has_le.le, has_mul.mul, has_inv.inv, has_zero.zero],
+     have : T+{l ⩑ ¬̇l} ⊢̇ l ⩑ ¬̇l, simp[-provable.and], simp at this,
+     refine provable.deduction.mp (provable.explosion this.1 this.2) }
+
+private lemma top_le_sup_compl (l : Lindenbaum T) : 1 ≤ l + l⁻¹ :=
+by induction l using fopl.Lindenbaum.ind_on; simp[has_le.le, has_add.add, has_inv.inv, has_one.one, form.or]
+
+instance : boolean_algebra (Lindenbaum T) :=
+{ bot := 0,
+  top := 1,
+  le  := (≤),
+  lt  := (<),
+  sup := (+),
+  inf := (*),
+  compl := (λ l, l⁻¹),
+  sdiff := (λ l m, l * m⁻¹),
+  le_refl := λ l, by induction l using fopl.Lindenbaum.ind_on; simp[has_le.le],
+  le_trans := λ l m n,
+  by { induction l using fopl.Lindenbaum.ind_on,
+       induction m using fopl.Lindenbaum.ind_on,
+       induction n using fopl.Lindenbaum.ind_on, simp[has_le.le], refine provable.imp_trans },
+  lt_iff_le_not_le := λ l m,
+  by { induction l using fopl.Lindenbaum.ind_on,
+       induction m using fopl.Lindenbaum.ind_on, simp[has_le.le, has_lt.lt] },
+  le_antisymm := λ l m, le_antisymm,
+  bot_le := zero_minimum,
+  le_sup_left := λ l m, by { induction l using fopl.Lindenbaum.ind_on, induction m using fopl.Lindenbaum.ind_on,
+     simp[has_add.add, has_le.le, preorder.le, provable.or_l] },
+  le_sup_right := λ l m, by { induction l using fopl.Lindenbaum.ind_on, induction m using fopl.Lindenbaum.ind_on,
+     simp[has_add.add, has_le.le, preorder.le, provable.or_r] },
+  sup_le := λ _ _ _, sup_le,
+  inf_le_left := λ l m, by { induction l using fopl.Lindenbaum.ind_on,
+    induction m using fopl.Lindenbaum.ind_on, simp[has_le.le, has_mul.mul, preorder.le],
+    refine provable.hyp_and_left (by simp) },
+  inf_le_right := λ l m, by { induction l using fopl.Lindenbaum.ind_on,
+    induction m using fopl.Lindenbaum.ind_on, simp[has_le.le, has_mul.mul, preorder.le],
+    refine provable.hyp_and_right (by simp) },
+  le_inf := λ _ _ _, le_inf,
+  le_sup_inf := λ _ _ _, le_sup_inf,
+  sup_inf_sdiff := sup_inf_sdiff,
+  inf_inf_sdiff := inf_inf_sdiff,
+  le_top := one_maximum,
+  inf_compl_le_bot := inf_compl_le_bot,
+  top_le_sup_compl := top_le_sup_compl,
+  sdiff_eq := λ _ _, rfl }
 
 end Lindenbaum
 
